

Chapter 2

Vector spaces

$\mathbb{K} = \mathbb{R}$ or \mathbb{C} .

2.1 Definitions

2.1.1 Vector spaces

Definition 1

E is a \mathbb{K} -vector space if E is equipped with a law of internal product denoted $+$ and of a law of external product (of $\mathbb{K} \times E$ in E) denoted \cdot such that

- $(E, +)$ is a commutative group
- $\forall (\lambda, \mu) \in \mathbb{K}^2, \forall (x, y) \in E^2$

$$\cdot (\lambda + \mu).x = \lambda.x + \mu.x$$

$$\cdot \lambda.(x + y) = \lambda.x + \lambda.y$$

$$\cdot \lambda.(\mu.x) = (\lambda\mu).x$$

$$\cdot 1.x = x$$

Examples

1. For all $n \in \mathbb{N}^*$, \mathbb{R}^n is a \mathbb{R} -vector space.

2. The space of polynomials with real coefficients $\mathbb{R}[X]$ is a \mathbb{R} -vector space.
3. The space of functions from \mathbb{R} to \mathbb{R} is a \mathbb{R} -vector space.
4. The space of real sequences $\mathbb{R}^{\mathbb{N}}$ is a \mathbb{R} -vector space.

2.1.2 Vector subspaces

Definition 2

Let E be a \mathbb{K} -vector space. F is a vector subspace of E if

- $F \subset E$
- $F \neq \emptyset$
- $\forall (x, y) \in F^2, \forall (\lambda, \mu) \in \mathbb{K}^2, \lambda x + \mu y \in F$

Remark

To prove that a set is vectorial, we show in almost all the cases that it is a vector subspace of a classical vector space such as one of the examples above.

Examples

1. Let $n \in \mathbb{N}$. The space of polynomials of degree less than or equal to n with real coefficients is a \mathbb{R} -vector space as it is a vector subspace of the \mathbb{R} -vector space $\mathbb{R}[X]$.
2. The set of functions even from \mathbb{R} to \mathbb{R} is a \mathbb{R} -vector space as it is a vector subspace of the \mathbb{R} -vector space $\mathbb{R}^{\mathbb{R}}$.
3. The set of continuous functions from \mathbb{R} to \mathbb{R} is a \mathbb{R} -vector space as it is a vector subspace of the \mathbb{R} -vector space $\mathbb{R}^{\mathbb{R}}$.

2.2 Operations

2.2.1 Intersection of vector subspaces

Proposition 1

Let E be a \mathbb{K} -vector space, F and G be two vector subspaces of E . Then $F \cap G$ is a vector subspace of E . More generally, if $(F_i)_{i \in I}$ is a family of vector subspaces of E , then $\bigcap_{i \in I} F_i$ is a vector subspace of E .

Remark

This proposition is essential for the notion of spanned vector subspace.

2.2.2 Sum of vector subspaces

Definition 3

Let E be a \mathbb{K} -vector space, F and G be two vector subspaces of E .

We define the set $F + G$ by

$$F + G = \{z \in E, \exists (x, y) \in F \times G, z = x + y\}$$

Proposition 2

Let E be a \mathbb{K} -vector space, F and G two vector subspaces of E . Then $F + G$ is a vector subspace of E .

2.3 Supplementary subspaces

2.3.1 Vector subspaces in direct sum

Definition 4

Let F and G be two vector subspaces of a \mathbb{K} -vector space E . We say that F and G are in direct sum if

$$\forall (x, y) \in F \times G : x + y = 0 \implies x = y = 0$$

Example

In \mathbb{R}^3 , the vector subspaces $\mathbb{R} \times \{0\} \times \{0\}$ and $\{0\} \times \mathbb{R} \times \{0\}$ are in direct sum.

Proposition 3

The following assertions are equivalent :

- (i) F and G are in direct sum
- (ii) $F \cap G = \{0\}$
- (iii) $\forall x \in F + G, \exists!(y, z) \in F \times G, x = y + z$

2.3.2 Supplementary subspaces**Definition 5**

Let F and G be two vector subspaces of a \mathbb{K} -vector space E . We say that F and G are supplementary in E and we write $E = F \oplus G$ if

$$F \cap G = \{0\} \quad \text{and} \quad E = F + G$$

Proposition 4

Let E be a \mathbb{K} -vector space, F and G two vector subspaces of E . Then

$$E = F \oplus G \iff \forall x \in E, \exists!(y, z) \in F \times G, x = y + z$$

Example

Let $E = \mathbb{R}^{\mathbb{R}}$, $P = \{f \in \mathbb{R}^{\mathbb{R}}, f \text{ even}\}$ and $I = \{f \in \mathbb{R}^{\mathbb{R}}, f \text{ odd}\}$. Then P and I are supplementary in E .

2.4 Spanned vector subspace**Definition 6**

Let E be a \mathbb{K} -vector space and $X \subset E$. there exists a smallest vector subspace of E containing X . It is the intersection of all the vector subspaces of E containing X . It is called vector subspace of E spanned by X and noted $\text{Span}(X)$.

Proposition 5

Let E be a \mathbb{K} -vector space and $X = \{x_1, \dots, x_n\} \subset E$. Then

$$\text{Span}(X) = \{\lambda_1 x_1 + \dots + \lambda_n x_n; (\lambda_1, \dots, \lambda_n) \in \mathbb{K}^n\}$$

Examples

1. In the plan $E = \mathbb{R}^2$, the vector subspace spanned by a non null vector x of E is $\text{Span}(\{x\}) = \mathbb{R}x$ i.e. the vectorial line spanned par x .
2. In the plan $E = \mathbb{R}^2$, the vector subspace spanned by two non null and non collinear vectors of E is whole E .

2.5 Linear map

2.5.1 Definition

Definition 7

Let E, F be two \mathbb{K} -vector spaces and $f : E \rightarrow F$. We say that f is linear (and we write $f \in \mathcal{L}(E, F)$) if

$$\forall (x, y) \in E^2, \forall (\lambda, \mu) \in \mathbb{K}^2, \quad f(\lambda x + \mu y) = \lambda f(x) + \mu f(y)$$

Examples

1. $I : \begin{cases} C^0(\mathbb{R}, \mathbb{R}) & \longrightarrow \mathbb{R} \\ f & \longmapsto \int_a^b f(x) dx \end{cases}$ is linear.
2. $D : \begin{cases} \mathbb{R}[X] & \longrightarrow \mathbb{R}[X] \\ P & \longmapsto P' \end{cases}$ is linear.

Proposition 6

1. $\mathcal{L}(E, F)$ is a \mathbb{K} -vector space
2. Let $f \in \mathcal{L}(E, F)$. Then
 - a. $f(0) = 0$
 - b. $\forall (x, y) \in E^2, \quad f(x - y) = f(x) - f(y)$

2.5.2 Kernel and image

Definition 8

Let $f \in \mathcal{L}(E, F)$.

We call kernel (resp. image) of f the set denoted $\text{Ker}(f) = \{x \in E, f(x) = 0\}$ (resp. $\text{Im}(f) = \{f(x); x \in E\}$).

Proposition 7

Let $f \in \mathcal{L}(E, F)$.

1. $\text{Ker}(f)$ and $\text{Im}(f)$ are respectively vector subspaces of E and F .
2. f injective $\iff \text{Ker}(f) = \{0\}$.
3. f surjective $\iff \text{Im}(f) = F$.

Example

Let us consider the linear map $f : \begin{cases} \mathbb{R}_n[X] & \longrightarrow \mathbb{R}_n[X] \\ P & \longmapsto P' \end{cases}$

then $\text{Ker}(f) = \{\text{constant polynomials}\}$ and $\text{Im}(f) = \mathbb{R}_{n-1}[X]$.

2.6 Basis and dimension

2.6.1 Linearly independent family, spanning family, basis

Definition 9

Let E be a \mathbb{K} -vector space and $L = \{x_1, \dots, x_n\} \subset E$. We say that L is a linearly independent family if

$$\forall (\lambda_1, \dots, \lambda_n) \in \mathbb{K}^n : \lambda_1 x_1 + \dots + \lambda_n x_n = 0 \implies (\lambda_1, \dots, \lambda_n) = (0, \dots, 0)$$

.

Definition 10

Let E be a \mathbb{K} -vector space and $G = \{x_1, \dots, x_n\} \subset E$. We say that G spans E (or that E is spanned by G or that G is a spanning part of E) if $E = \text{Vect}(G)$.

Definition 11

Let E be a \mathbb{K} -vector space and $B = \{x_1, \dots, x_n\} \subset E$. We say that B is a basis of E if B is linearly independent and spans E .

Example

$B = (1, X - 1, (X + 1)^2)$ is a basis of $\mathbb{R}_2[X]$.

2.6.2 Dimension**Definition 12**

Let E be a \mathbb{K} -vector space. We say that E is of finite dimension if it is spanned by a finite family of vectors of E .

Example

Let $n \in \mathbb{N}$. Then $\mathbb{R}_n[X]$ is of finite dimension as $\mathbb{R}_n[X] = \text{Vect}(1, X, X^2, \dots, X^n)$.

Theorem 1

Let E be a \mathbb{K} -vector space of finite dimension. All the basis of E have same cardinal. This number is called dimension of E and denoted $\dim_{\mathbb{K}}(E)$ yet $\dim(E)$.

Examples

1. Let $n \in \mathbb{N}$. Then $\mathbb{R}_n[X]$ is of dimension $n + 1$ as $B = (1, X, X^2, \dots, X^n)$ is a basis of E and $\text{Card}(B) = n + 1$.
2. $E = \mathbb{C}$ is a \mathbb{C} -vector space of dimension 1 as $B = \{1\}$ is a basis of E as a \mathbb{C} -vector space.
3. $F = \mathbb{C}$ is a \mathbb{R} -vector space of dimension 2 as $B = \{1, i\}$ is a basis of F as a \mathbb{R} -vector space.

2.6.3 The incomplete basis theorem and its corollaries

Theorem 2

Let E be a \mathbb{K} -vector space of finite dimension spanned by G . Let L be a linearly independent family of E . Then we can complete the family L by vectors taken in G to obtain a basis of E .

Proposition 8

Let E be a \mathbb{K} -vector space of finite dimension such that $E \neq \{0\}$. Then E admits at least one basis.

Proposition 9

Let E be a \mathbb{K} -vector space of finite dimension and F be a vector subspace of E . Then F admits at least one supplementary subspace in E .

Proposition 10

Let E be a \mathbb{K} -vector space of finite dimension, F and G two vector subspaces supplementary in E , B a basis of F and B' a basis of G .
then $B \sqcup B'$ is a basis of E .

Proposition 11

$$E = F \oplus G \implies \dim(E) = \dim(F) + \dim(G)$$

Proposition 12

Let E be a \mathbb{K} -vector space of finite dimension, F and G be two vector subspaces of E such that

$$F \subset G \quad \text{and} \quad \dim(F) = \dim(G)$$

Then $F = G$

Proposition 13

Let E and F be two \mathbb{K} -vector spaces of finite dimension. Then

$$f \in \mathcal{L}(E, F) \quad \text{bijective} \implies \dim(E) = \dim(F)$$

2.6.4 Rank-nullity theorem

Theorem 3

Let $f \in \mathcal{L}(E, F)$ where E is of finite dimension. Then

$$\dim(E) = \dim(\text{Ker}(f)) + \dim(\text{Im}(f))$$

Proposition 14

Let E be a \mathbb{K} -vector space of finite dimension, F and G be two vector subspaces of E . Then

$$\dim(F + G) = \dim(F) + \dim(G) - \dim(F \cap G)$$

2.7 Standard exercises

Exercise 1

Let E be a \mathbb{K} -vector space of finite dimension n which is even and $f \in \mathcal{L}(E)$. Prove that

$$(f^2 = 0 \text{ and } \dim(\text{Im}(f)) = \frac{n}{2}) \iff (\text{Im}(f) = \text{Ker}(f))$$

Solution

$\boxed{\implies}$ Let us prove that $\text{Im}(f) \subset \text{Ker}(f)$.

Let $y \in \text{Im}(f)$. Then there exists $x \in E$ such that $y = f(x)$. Yet $f^2 = 0$ so $f(y) = f^2(x) = 0$ so $y \in \text{Ker}(f)$.

On the other hand, using the Rank-nullity theorem, $\dim(\text{Ker}(f)) + \dim(\text{Im}(f)) = n$ or $\dim(\text{Im}(f)) = \frac{n}{2}$ thus $\dim(\text{Ker}(f)) = \frac{n}{2}$.

Hence $\dim(\text{Im}(f)) = \dim(\text{Ker}(f))$.

As $\text{Im}(f) \subset \text{Ker}(f)$, we deduce that $\text{Im}(f) = \text{Ker}(f)$.

$\boxed{\impliedby}$ Let us prove that $f^2 = 0$.

Let $x \in E$. Then $f(x) \in \text{Im}(f)$ yet $\text{Im}(f) = \text{Ker}(f)$ so $f(x) \in \text{Ker}(f)$ i.e. $f^2(x) = 0$.

On the other hand, using the Rank-nullity theorem, we have $\dim(\text{Ker}(f)) + \dim(\text{Im}(f)) = n$ yet $\text{Im}(f) = \text{Ker}(f)$

so $\dim(\text{Im}(f)) = \frac{n}{2}$.

Exercise 2

Let E be a \mathbb{R} -vector space and $(f, g) \in \mathcal{L}(E) \times \mathcal{L}(E)$.

1. Prove that $(\text{Ker}(g \circ f) = \text{Ker}(f)) \iff (\text{Ker}(g) \cap \text{Im}(f) = \{0\})$
2. Prove that $(\text{Im}(g \circ f) = \text{Im}(g)) \iff (\text{Ker}(g) + \text{Im}(f) = E)$

Solution

1. $\boxed{\implies}$

Let us assume $\text{Ker}(g \circ f) = \text{Ker}(f)$.

Let $y \in \text{Ker}(g) \cap \text{Im}(f)$. Then there exists $x \in E$ such that $y = f(x)$ and $g(y) = 0$. Hence $g(f(x)) = 0$ i.e. $x \in \text{Ker}(g \circ f)$. Yet

$$\text{Ker}(g \circ f) = \text{Ker}(f)$$

So $x \in \text{Ker}(f)$ so $y = f(x) = 0$. Hence $\text{Ker}(g) \cap \text{Im}(f) = \{0\}$ (the other inclusion being trivial).

$\boxed{\impliedby}$

Let us assume $\text{Ker}(g) \cap \text{Im}(f) = \{0\}$.

Let us prove first that $\text{Ker}(g \circ f) \subset \text{Ker}(f)$.

Let $x \in \text{Ker}(g \circ f)$. Then $g(f(x)) = 0$. So $f(x) \in \text{Ker}(g)$ and $f(x) \in \text{Im}(f)$.

Thus $f(x) \in \text{Ker}(g) \cap \text{Im}(f)$. Yet

$$\text{Ker}(g) \cap \text{Im}(f) = \{0\}$$

so $f(x) = 0$ i.e. $x \in \text{Ker}(f)$.

Let us prove now that $\text{Ker}(f) \subset \text{Ker}(g \circ f)$.

Let $x \in \text{Ker}(f)$. Then $f(x) = 0$. So $g(f(x)) = g(0) = 0$ so $x \in \text{Ker}(g \circ f)$.

2. $\boxed{\implies}$

Let us assume $\text{Im}(g \circ f) = \text{Im}(g)$.

Let us prove that $E \subset \text{Ker}(g) + \text{Im}(f)$.

Let $x \in E$. Then $g(x) \in \text{Im}(g) = \text{Im}(g \circ f)$. So there exists $z \in E$ such that $g(x) = g(f(z))$. Hence $x = x - f(z) + f(z)$ where $f(z) \in \text{Im}(f)$ and $x - f(z) \in \text{Ker}(g)$ as

$$g(x - f(z)) = g(x) - g(f(z)) = 0$$

So $x \in \text{Ker}(g) + \text{Im}(f)$. Hence $E = \text{Ker}(g) + \text{Im}(f)$ (the other inclusion being trivial).



Let us assume $E = \text{Ker}(g) + \text{Im}(f)$.

The inclusion $\text{Im}(g \circ f) \subset \text{Im}(g)$ is trivial.

Let us prove that $\text{Im}(g) \subset \text{Im}(g \circ f)$.

Let $y \in \text{Im}(g)$. Then there exists $x \in E$ such that $y = g(x)$. Yet

$$E = \text{Ker}(g) + \text{Im}(f)$$

so $x = x_1 + x_2$ where $(x_1, x_2) \in \text{Ker}(g) \times \text{Im}(f)$. Hence

$$y = g(x) = g(x_1 + x_2) = g(x_2)$$

Yet, $x_2 \in \text{Im}(f)$ so there exists $z \in E$ such that $x_2 = f(z)$. Hence

$$y = g(f(z))$$

So $y \in \text{Im}(g \circ f)$. Thus $\text{Im}(g) \subset \text{Im}(g \circ f)$.

Exercise 3

Let E be a \mathbb{R} -vector space, $(f, g, h) \in \mathcal{L}(E) \times \mathcal{L}(E) \times \mathcal{L}(E)$. Prove that

$$\text{Im}(h \circ f) \subset \text{Im}(h \circ g) \iff \text{Im}(f) + \text{Ker}(h) \subset \text{Im}(g) + \text{Ker}(h)$$

Solution



Let us assume $\text{Im}(h \circ f) \subset \text{Im}(h \circ g)$.

Let $y \in \text{Im}(f) + \text{Ker}(h)$. Then there exists $(x, z) \in E \times \text{Ker}(h)$ such that $y = f(x) + z$. So

$$h(y) = h(f(x) + z) = h(f(x)) \in \text{Im}(h \circ f) \subset \text{Im}(h \circ g)$$

Hence there exists $t \in E$ such that $h(y) = h(g(t))$. So

$$y = g(t) + y - g(t) \in \text{Im}(g) + \text{Ker}(h)$$

as

$$h(y - g(t)) = h(y) - h(g(t)) = 0$$

Hence $\text{Im}(f) + \text{Ker}(h) \subset \text{Im}(g) + \text{Ker}(h)$.



Let us assume $\text{Im}(f) + \text{Ker}(h) \subset \text{Im}(g) + \text{Ker}(h)$.

Let $y \in \text{Im}(h \circ f)$. Then there exists $x \in E$ such that $y = h(f(x))$. Yet

$$f(x) \in \text{Im}(f) \subset \text{Im}(f) + \text{Ker}(h) \subset \text{Im}(g) + \text{Ker}(h)$$

Thus there exists $(u, v) \in E \times \text{Ker}(h)$ such that $f(x) = g(u) + v$. Hence

$$y = h(g(u) + v) = h(g(u)) \in \text{Im}(h \circ g)$$

Thus $\text{Im}(h \circ f) \subset \text{Im}(h \circ g)$.

Exercise 4

Let E be a \mathbb{K} -vector space and $(p, q) \in \mathcal{L}(E) \times \mathcal{L}(E)$ be such that $p^2 = p$ and $q^2 = q$ (i.e. p and q are projectors). We assume $p \neq 0$, $q \neq 0$ and $p \neq q$.

1. Let $\alpha \in \mathbb{R}$. Prove that $q = \alpha p \Rightarrow \alpha p = \alpha^2 p$.
2. Prove that (p, q) forms a linearly independent family in $\mathcal{L}(E)$.

Solution

1. Let us assume $q = \alpha p$. Then $\alpha p = q^2$ (as $q = q^2$) so $\alpha p = (\alpha p)^2$ (as $q = \alpha p$) i.e. $\alpha p = \alpha^2 p^2$
Let $\alpha p = \alpha^2 p$ (as $p^2 = p$).
2. We use a proof by contradiction. We assume that (p, q) are linearly dependent i.e. p and q are collinear.
Then $q = \alpha p$ where $\alpha \in \mathbb{R}$.

Using question 1., we have $\alpha p = \alpha^2 p$ Let $(\alpha^2 - \alpha)p = 0$ i.e. $\alpha(\alpha - 1)p = 0$ then $\alpha(\alpha - 1) = 0$ as $p \neq 0$. So $\alpha = 0$ or $\alpha = 1$.

Yet, if $\alpha = 0$ then $q = 0$ which contradicts the hypothesis. Similarly, if $\alpha = 1$ then $q = p$ which also contradicts the hypothesis.